Allow memoizing dependently typed functions

MemoNat.lean
@@ -23,21 +23,64 @@ protected def empty {α} (cap : Nat) : SArray α 0 := ⟨Array.mkEmpty cap, rfl�
 
 end SArray
 
+inductive Any.{u} : Type u
+| mk {α : Sort u} : α → Any
+
+protected abbrev Any.Sort : Any → Sort _
+| @mk α _ => α
+
+protected abbrev Any.val : (a : Any) → a.Sort
+| mk x => x
+
+def DArray (n : Nat) (C : Nat → Type _) :=
+  {a : SArray Any n // ∀ (i : Fin n), (a.get i).Sort = C i }
+
+namespace DArray
+
+protected def push {n C} (a : DArray n C) (x : C n) : DArray (n + 1) C :=
+  ⟨a.1.push (Any.mk x), by 
+    intro ⟨i, hi⟩
+    rewrite [SArray.get_push]
+    split
+    case inl hi2 => apply a.2
+    case inr hi2 =>
+      have : i = n := Nat.le_antisymm (Nat.le_of_lt_succ hi) (Nat.le_of_not_lt hi2)
+      cases this
+      rfl
+  ⟩
+
+protected def get {n C} (a : DArray n C) (i : Fin n) : C i :=
+  a.2 i ▸ (a.1.get i).val
+
+protected theorem get_push {n C} (a : DArray n C) (x : C n) (i : Nat) (hi : i < n + 1) :
+    (a.push x).get ⟨i, hi⟩ =
+      if h : i < n
+      then a.get ⟨i, h⟩
+      else (Nat.le_antisymm (Nat.le_of_lt_succ hi) (Nat.le_of_not_lt h) ▸ x : C i) := by
+  unfold DArray.push
+  unfold DArray.get
+  -- rw [ SArray.get_push a.1 (Any.mk x) i hi ]
+  sorry
+  
+protected def empty {C} (cap : Nat) : DArray 0 C := ⟨SArray.empty cap, λ i => Fin.elim0 i⟩
+
+end DArray
+
 namespace NatMemo
 
-protected def memoVec {α} (cap : Nat) (f : (n : Nat) → (∀ i, i < n → α) → α ) :
-  (n : Nat) → SArray α n
+protected def memoVec {C} (cap : Nat) (f : (n : Nat) → (∀ i, i < n → C i) → C n) :
+  (n : Nat) → DArray n C
   | 0 => .empty cap
   | n + 1 =>
     let v := NatMemo.memoVec cap f n
     v.push (f n (fun i ih => v.get ⟨i, ih⟩))
 
-def memo {α : Type} (f : (n : Nat) → (∀ i, i < n → α) → α) (n : Nat) : α :=
+def memo {C : Nat → Sort _} (f : (n : Nat) → (∀ i, i < n → C i) → C n) (n : Nat) : C n :=
   (NatMemo.memoVec (n + 1) f (n + 1)).get ⟨n, Nat.le_refl _⟩
 
-theorem memoVec_spec {α}
-  (g : Nat → α)
-  (f : (n : Nat) → (∀ i, i < n → α) → α)
+theorem memoVec_spec {C : Nat → Sort _}
+  (g : ∀ n, C n)
+  (f : (n : Nat) → (∀ i, i < n → C i) → C n)
   (h : ∀ n, f n (fun i _ => g i) = g n)
   n : ∀ c i hi, (NatMemo.memoVec c f n).get ⟨i, hi⟩ = g i := by
     induction n
@@ -47,7 +90,7 @@ theorem memoVec_spec {α}
     case succ n ih =>
       intro c i hi
       rw [NatMemo.memoVec]
-      apply Eq.trans (SArray.get_push _ _ _ _)
+      apply Eq.trans (DArray.get_push _ _ _ _)
       split
       case inl hn =>
         apply ih
@@ -55,12 +98,13 @@ theorem memoVec_spec {α}
         have i_eq_n : i = n := Nat.le_antisymm (Nat.lt_succ.1 hi) (Nat.not_lt.1 hn)
         rcases i_eq_n
         rw [<- h]
+        simp only
         congr with i hi'
         apply ih
 
-theorem memo_spec {α}
-  (g : Nat → α)
-  (f : (n : Nat) → (∀ i, i < n → α) → α)
+theorem memo_spec {C : Nat → Sort _}
+  (g : ∀ n, C n)
+  (f : (n : Nat) → (∀ i, i < n → C i) → C n)
   (h : ∀ n, f n (fun i _ => g i) = g n) :
   g = memo f := funext (fun _ => (memoVec_spec g f h _ _ _ _).symm)
 
